updates

Veritas.Verifier.Blum.fst
@@ -2,263 +2,175 @@ module Veritas.Verifier.Blum
 
 open Veritas.EAC
 
+module S = FStar.Seq
+module SA = Veritas.SeqAux
 module E = Veritas.EAC
 module VT = Veritas.Verifier.Thread
 
-(* get the add seq of a log *)
-let rec add_seq (il:VT.verifiable_log): 
-  Tot (seq ms_hashfn_dom)
-  (decreases (VT.length il)) =
-  let (id,l) = il in
-  let n = length l in  
-  if n = 0 then 
-    Seq.empty #ms_hashfn_dom
-  else 
-    let l' = hprefix l in
-    let e = telem l in
-    match e with
-    | AddB r t j -> append1 (add_seq (id, l')) (MHDom r t j)
-    | _ ->  add_seq (id,l')
+let rec ts_add_seq_aux (itsl: its_log): 
+  Tot (seq ms_hashfn_dom) 
+  (decreases (I.length itsl)) = 
+  let n = I.length itsl in
+  if n = 0 then S.empty #ms_hashfn_dom
+  else
+    let itsl' = I.prefix itsl (n - 1) in
+    let s' = ts_add_seq_aux itsl' in
+    let e = I.index itsl (n - 1) in
+    if is_blum_add e then 
+      SA.append1 s' (blum_add_elem e)
+    else
+      s'
+  
+let ts_add_seq = ts_add_seq_aux
 
-(* get the add multi-set of a log *)
-let add_set (il:VT.verifiable_log): mset ms_hashfn_dom = 
-  seq2mset (add_seq il)
-
-(* 
- * the hadd hash value maintained by a verifier thread is the multiset hash 
- * of its add_set 
- *)
-let rec lemma_hadd_add_set (il:VT.verifiable_log):
-  Lemma (requires True)
-        (ensures (thread_hadd (t_verify (fst il) (snd il)) = ms_hashfn (add_seq il))) 
-        (decreases (VT.length il)) =
-  let (id,l) = il in
-  let n = length l in
-  let st = t_verify id l in
-  if n = 0 then 
-    lemma_hashfn_empty()  
+let rec lemma_add_elem_correct_aux (itsl: its_log) (i: I.seq_index itsl):
+  Lemma (requires (is_blum_add (I.index itsl i)))
+        (ensures (contains (blum_add_elem (I.index itsl i)) (ts_add_set itsl)))
+        (decreases (I.length itsl)) =
+  let n = I.length itsl in
+  if n = 0 then ()
   else (
-    let l' = hprefix l in
-    let e = telem l in
-    lemma_hadd_add_set (id, l');
-    match e with
-    | AddB r t j -> 
-           lemma_hashfn_app (add_seq (id, l')) (MHDom r t j)
-    | _ -> ()
+    let itsl' = I.prefix itsl (n - 1) in
+    assert(TL.verifiable itsl');   
+    let s' = ts_add_seq_aux itsl' in
+    let e = I.index itsl (n - 1) in    
+    if i < n- 1 then (
+      assert(I.index itsl i = I.index itsl' i);
+      lemma_add_elem_correct_aux itsl' i;
+      admit()
+    )
+    else
+      admit()
   )
 
-(* concatenation of all local add-seq *)
-let g_add_seq (gl: VG.verifiable_log): seq (ms_hashfn_dom) = 
-  let gl' = verifiable_threads gl in
-  (* sequence of local add_sequences *)
-  let l_adds = map add_seq gl' in
-  reduce (Seq.empty #ms_hashfn_dom) append l_adds
 
-(* the hadd that the verifier computes is the multiset hash of all the adds *)
-let lemma_g_hadd_correct (gl: VG.verifiable_log):
-  Lemma (VG.hadd gl = ms_hashfn (g_add_seq gl)) = admit()
+let lemma_add_elem_correct (itsl: its_log) (i: I.seq_index itsl):
+  Lemma (requires (is_blum_add (I.index itsl i)))
+        (ensures (contains (blum_add_elem (I.index itsl i)) (ts_add_set itsl))) = 
+  admit()
 
-(* sequence of versioned records evicted from a verifier *)
-let rec evict_seq (il:VT.verifiable_log):
-  Tot (seq ms_hashfn_dom)
-  (decreases (VT.length il)) = 
-  let (id,l) = il in
-  let n = length l in  
-  if n = 0 then 
-    Seq.empty #ms_hashfn_dom
-  else 
-    let (_,l') = VT.prefix il (n - 1) in
-    let e = telem l in
-    let vs' = t_verify id l' in
-    let st' = thread_store vs' in
-    match e with
-    | EvictB k t -> 
-      let v = stored_value st' k in 
-      append1 (evict_seq (id, l')) (MHDom (k,v) t id)
-    | EvictBM k k' t -> 
-      let v = stored_value st' k in 
-      append1 (evict_seq (id, l')) (MHDom (k,v) t id)    
-    | _ -> evict_seq (id, l')
+let ts_add_seq_key (itsl: its_log) (k:key): seq ms_hashfn_dom = admit()
 
-(* evict multiset of a verifier *)
-let evict_set (il:VT.verifiable_log): mset ms_hashfn_dom =
-  seq2mset (evict_seq il)
+let lemma_ts_add_set_correct (itsl: its_log): 
+  Lemma (ts_add_set itsl == g_add_set (g_vlog_of itsl)) = admit()
 
-(* a single sequence containing all the blum evicts *)
-let g_evict_seq (gl: VG.verifiable_log): seq ms_hashfn_dom = 
-  let gl' = verifiable_threads gl in
-  (* sequence of local add_sequences *)
-  let l_evicts = map evict_seq gl' in
-  reduce (Seq.empty #ms_hashfn_dom) append l_evicts 
+let lemma_ts_add_set_key_extend (itsl: its_log {I.length itsl > 0}):
+  Lemma (requires (is_blum_add (I.telem itsl)))
+        (ensures (ts_add_set_key itsl (key_of (I.index itsl (I.length itsl - 1))) == 
+                  add_elem (ts_add_set_key (I.prefix itsl (I.length itsl - 1))
+                                           (key_of (I.index itsl (I.length itsl - 1))))
+                           (blum_add_elem (I.telem itsl)))) = admit()
 
-let g_evict_set_is_set (gl: VG.verifiable_log): 
-  Lemma (is_set (g_evict_set gl)) = admit()
+let lemma_ts_add_set_contains_add_elem (itsl: its_log) (i:I.seq_index itsl):
+  Lemma (requires (is_blum_add (I.index itsl i)))
+        (ensures (MS.contains (blum_add_elem (I.index itsl i)) (ts_add_set itsl))) = admit()
 
-let lemma_ghevict_correct (gl: VG.verifiable_log):
-  Lemma (VG.hevict gl = ms_hashfn (g_evict_seq gl)) = admit()
-
-let rec lemma_hevict_evict_set (il:VT.verifiable_log):
-  Lemma (requires True)
-        (ensures (thread_hevict (t_verify (fst il) (snd il)) = ms_hashfn (evict_seq il)))
-        (decreases (VT.length il)) =
-  let (id, l) = il in
-  let n = length l in
-  if n = 0 then lemma_hashfn_empty()
-  else (
-    let l' = hprefix l in
-    let e = telem l in
-    let vs' = t_verify id l' in
-    let st' = thread_store vs' in    
-    lemma_hevict_evict_set (id, l');
-    VT.lemma_thread_id_state (id, l');
-    match e with
-    | EvictB k t -> 
-      let v = stored_value st' k in
-      lemma_hashfn_app (evict_seq (id, l')) (MHDom (k,v) t id)
-    | EvictBM k _ t -> 
-      let v = stored_value st' k in
-      lemma_hashfn_app (evict_seq (id, l')) (MHDom (k,v) t id)
-    | _ -> ()
-  )
-
-let lemma_add_elem_correct (#n:pos) (itsl: its_log n) (i:seq_index itsl{is_blum_add (index itsl i)}):
-  Lemma (requires (is_blum_add (index itsl i)))
-        (ensures (contains (blum_add_elem (index itsl i)) (ts_add_set itsl))) = admit()
-
-
-let ts_add_seq_key (#n:pos) (itsl: its_log n) (k:key): seq ms_hashfn_dom
- = admit()
-
-let lemma_ts_add_set_correct (#n:pos) (itsl: its_log n): 
-  Lemma (ts_add_set itsl == g_add_set (partition_idx_seq itsl)) = admit()
-
-let lemma_ts_add_set_key_extend (#n:pos) (itsl: its_log n {length itsl > 0}):
-  Lemma (requires (is_blum_add (telem itsl)))
-        (ensures (ts_add_set_key itsl (key_of (index itsl (length itsl - 1))) == 
-                  add_elem (ts_add_set_key (prefix itsl (length itsl - 1))
-                                           (key_of (index itsl (length itsl - 1))))
-                           (blum_add_elem (telem itsl)))) = admit()
-
-let lemma_ts_add_set_contains_add_elem (#n:pos) (itsl: its_log n) (i:seq_index itsl):
-  Lemma (requires (is_blum_add (index itsl i)))
-        (ensures (MS.contains (blum_add_elem (index itsl i)) (ts_add_set itsl))) = admit()
-
-let lemma_ts_add_set_key_contains_only (#p:pos) (itsl: its_log p) (k:key) (be: ms_hashfn_dom):
+let lemma_ts_add_set_key_contains_only (itsl: its_log) (k:key) (be: ms_hashfn_dom):
   Lemma (requires (MS.contains be (ts_add_set_key itsl k)))
         (ensures (MH.key_of be = k)) = admit()
 
-let some_add_elem_idx (#p:pos) (itsl: its_log p) 
+let some_add_elem_idx (itsl: its_log) 
   (be: ms_hashfn_dom{MS.contains be (ts_add_set itsl)}): 
-  (i:(seq_index itsl){is_blum_add (index itsl i) /\
-                      be = blum_add_elem (index itsl i)}) = admit()
+  (i:(I.seq_index itsl){is_blum_add (I.index itsl i) /\
+                      be = blum_add_elem (I.index itsl i)}) = admit()
+
+(* get the blum evict element from an index *)
+let blum_evict_elem (itsl: its_log) (i:I.seq_index itsl{is_evict_to_blum (I.index itsl i)}):
+  (e:ms_hashfn_dom{MH.key_of e = key_of (I.index itsl i)}) = admit()
+
+let lemma_index_blum_evict_prefix (itsl: its_log) (i:nat{i <= I.length itsl}) (j:nat{j < i}):
+  Lemma (requires (is_evict_to_blum (I.index itsl j)))
+        (ensures (blum_evict_elem itsl j = blum_evict_elem (I.prefix itsl i) j))
+        [SMTPat (blum_evict_elem (I.prefix itsl i) j)] = admit()
 
 
-let blum_evict_elem (#p:pos) (itsl: its_log p) (i:seq_index itsl{is_blum_evict (index itsl i)}):
-  (e:ms_hashfn_dom{MH.key_of e = TL.key_of (index itsl i)}) =
-  let (e,id) = index itsl i in
-  let tsle = time_seq_ext itsl in
-  assert(project_seq itsl = to_vlog tsle);
-  lemma_project_seq_index itsl i;
-  assert(to_vlog_entry (index tsle i) = e);
-  match e with
-  | EvictB k t -> 
-    let v = value_ext (index tsle i) in
-    MHDom (k,v) t id
-  | EvictBM k _ t -> 
-    let v = value_ext (index tsle i) in
-    MHDom (k,v) t id
+(* sequence of evicts in time sequence log *)
+let ts_evict_seq (itsl: its_log): seq ms_hashfn_dom = admit()
 
-let lemma_index_blum_evict_prefix (#p:pos) (itsl: its_log p) (i:nat{i <= length itsl}) (j:nat{j < i}):
-  Lemma (requires (is_blum_evict (index itsl j)))
-        (ensures (blum_evict_elem itsl j = blum_evict_elem (prefix itsl i) j))
-        [SMTPat (blum_evict_elem (prefix itsl i) j)] = admit()
+(* the evict sequence restricted to key k *)
+let ts_evict_seq_key (itsl: its_log) (k:key): seq ms_hashfn_dom = admit()
 
+(* the blum evicts in time sequenced log should be the same as global evict set *)
+let lemma_ts_evict_set_correct (itsl: its_log):
+  Lemma (ts_evict_set itsl == g_evict_set (g_vlog_of itsl)) = admit()
 
-let rec ts_evict_seq_aux (#n:pos) (itsl: its_log n): Tot (seq ms_hashfn_dom) 
-  (decreases (length itsl)) =
-  let m = length itsl in 
-  if m = 0 then Seq.empty #ms_hashfn_dom
-  else if is_blum_evict (index itsl (m - 1)) then
-    append1 (ts_evict_seq_aux (prefix itsl (m - 1))) (blum_evict_elem itsl (m - 1))   
-  else
-    ts_evict_seq_aux (prefix itsl (m - 1))
+(* if the tail element is not an evict, the evict set is the same as the evict 
+ * set of the length - 1 prefix 
+ *)
+let lemma_ts_evict_set_key_extend2 (itsl: its_log {I.length itsl > 0}):
+  Lemma (requires (not (is_evict_to_blum (I.index itsl (I.length itsl - 1)))))
+        (ensures (ts_evict_set_key itsl (key_of (I.index itsl (I.length itsl - 1))) == 
+                  ts_evict_set_key (I.prefix itsl (I.length itsl - 1))
+                                           (key_of (I.index itsl (I.length itsl - 1))))) = admit()
 
-let ts_evict_seq = ts_evict_seq_aux
-
-let ts_evict_seq_key (#n:pos) (itsl: its_log n) (k:key): seq ms_hashfn_dom = 
-  admit()
-
-let lemma_ts_evict_set_correct (#n:pos) (itsl: its_log n):
-  Lemma (ts_evict_set itsl == g_evict_set (partition_idx_seq itsl)) = admit()
-
-let lemma_ts_evict_set_key_extend2 (#n:pos) (itsl: its_log n {length itsl > 0}):
-  Lemma (requires (not (is_blum_evict (index itsl (length itsl - 1)))))
-        (ensures (ts_evict_set_key itsl (key_of (index itsl (length itsl - 1))) == 
-                  ts_evict_set_key (prefix itsl (length itsl - 1))
-                                           (key_of (index itsl (length itsl - 1))))) = admit()
-
-
-let index_blum_evict (#p:pos) (itsl: its_log p) (e: ms_hashfn_dom {contains e (ts_evict_set itsl)}):
-  (i:seq_index itsl{is_blum_evict (index itsl i) /\ 
+(* since evict_set is a pure set (not a multiset) we can identify the unique index 
+ * for each element of the set *)
+let index_blum_evict (itsl: its_log) (e: ms_hashfn_dom {contains e (ts_evict_set itsl)}):
+  (i:I.seq_index itsl{is_evict_to_blum (I.index itsl i) /\ 
                     blum_evict_elem itsl i = e}) = admit()
 
-let lemma_evict_before_add (#p:pos) (itsl: its_log p) (i:seq_index itsl{is_blum_add (index itsl i)}):
+(* if the blum add occurs in the blum evict set, its index is earlier *)
+let lemma_evict_before_add (itsl: its_log) (i:I.seq_index itsl{is_blum_add (I.index itsl i)}):
   Lemma (requires True)
-        (ensures (not (contains (blum_add_elem (index itsl i)) (ts_evict_set itsl)) \/
-                  index_blum_evict itsl (blum_add_elem (index itsl i)) < i)) = admit()
+        (ensures (not (contains (blum_add_elem (I.index itsl i)) (ts_evict_set itsl)) \/
+                  index_blum_evict itsl (blum_add_elem (I.index itsl i)) < i)) = admit()
 
 (* a slightly different version of of the previous lemma - the count of an add element 
  * in the evict set is the same in the prefix as the full sequence *)
-let lemma_evict_before_add2 (#p:pos) (itsl: its_log p) (i:seq_index itsl{is_blum_add (index itsl i)}):
+let lemma_evict_before_add2 (itsl: its_log) (i:I.seq_index itsl{is_blum_add (I.index itsl i)}):
    Lemma (requires True)
-         (ensures (MS.mem (blum_add_elem (index itsl i)) (ts_evict_set itsl) =
-                   MS.mem (blum_add_elem (index itsl i)) (ts_evict_set (prefix itsl i)))) = admit()
+         (ensures (MS.mem (blum_add_elem (I.index itsl i)) (ts_evict_set itsl) =
+                   MS.mem (blum_add_elem (I.index itsl i)) (ts_evict_set (I.prefix itsl i)))) = admit()
 
-let lemma_evict_before_add3 (#p:pos) (itsl: its_log p) (i: seq_index itsl) (j:seq_index itsl):
-  Lemma (requires (is_blum_add (index itsl i) /\
-                   is_blum_evict (index itsl j) /\
-                   blum_add_elem (index itsl i) = blum_evict_elem itsl j))
+let lemma_evict_before_add3 (itsl: its_log) (i: I.seq_index itsl) (j:I.seq_index itsl):
+  Lemma (requires (is_blum_add (I.index itsl i) /\
+                   is_evict_to_blum (I.index itsl j) /\
+                   blum_add_elem (I.index itsl i) = blum_evict_elem itsl j))
         (ensures (j < i)) = admit()
 
-let lemma_evict_add_count_same (#p:pos) (itsl: eac_ts_log p) (k:key):
-  Lemma (requires (is_eac_state_instore itsl k))
+(* for an eac ts log, if the eac state of a key k is instore, the count of blum evicts 
+ * is the same of blum adds for that key *)
+let lemma_evict_add_count_same (itsl: TL.eac_log) (k:key):
+  Lemma (requires (TL.is_eac_state_instore itsl k))
         (ensures (MS.size (ts_add_set_key itsl k) = MS.size (ts_evict_set_key itsl k))) = admit()
 
 (* for an eac ts log, if the eac state of a key k is evicted to merkle, the count of blum evicts 
  * is the same of blum adds for that key *)
-let lemma_evict_add_count_same_evictedm (#p:pos) (itsl: eac_ts_log p) (k:key):
+let lemma_evict_add_count_same_evictedm (itsl: TL.eac_log) (k:key):
   Lemma (requires (is_eac_state_evicted_merkle itsl k))
         (ensures (MS.size (ts_add_set_key itsl k) = MS.size (ts_evict_set_key itsl k))) = admit()
 
-let lemma_mem_key_add_set_same (#p:pos) (itsl: its_log p) (be: ms_hashfn_dom):
+let lemma_mem_key_add_set_same (itsl: its_log) (be: ms_hashfn_dom):
   Lemma (mem be (ts_add_set itsl) = mem be (ts_add_set_key itsl (MH.key_of be))) = admit()
 
-let lemma_mem_key_evict_set_same (#p:pos) (itsl: its_log p) (be: ms_hashfn_dom):
-  Lemma (mem be (ts_evict_set itsl) = mem be (ts_evict_set_key itsl (MH.key_of be))) = admit()
+let lemma_mem_key_evict_set_same (itsl: its_log) (be: ms_hashfn_dom):
+  Lemma (mem be (ts_evict_set itsl) = mem be (ts_evict_set_key itsl (MH.key_of be))) =admit()
 
-let lemma_mem_monotonic (#p:pos) (be:ms_hashfn_dom) (itsl: its_log p) (i:nat{i <= length itsl}):
-  Lemma (mem be (ts_evict_set itsl) >= mem be (ts_evict_set (prefix itsl i)) /\
-         mem be (ts_add_set itsl) >= mem be (ts_add_set (prefix itsl i))) = admit()
+(* the count of an element can only decrease in a prefix of itsl *)
+let lemma_mem_monotonic (be:ms_hashfn_dom) (itsl: its_log) (i:nat{i <= I.length itsl}):
+  Lemma (mem be (ts_evict_set itsl) >= mem be (ts_evict_set (I.prefix itsl i)) /\
+         mem be (ts_add_set itsl) >= mem be (ts_add_set (I.prefix itsl i))) = admit()
 
-let lemma_blum_evict_add_same (#p:pos) (itsl: eac_ts_log p) (i:seq_index itsl):
-  Lemma (requires (TL.is_blum_evict (index itsl i) /\
-                   TL.has_next_add_of_key itsl i (TL.key_of (index itsl i))))
-        (ensures (TL.is_blum_add (index itsl (TL.next_add_of_key itsl i (TL.key_of (index itsl i)))) /\
+(* the next add of a blum evict is a blum add of the same "element" *)
+let lemma_blum_evict_add_same (itsl: TL.eac_log) (i:I.seq_index itsl):
+  Lemma (requires (is_evict_to_blum (I.index itsl i) /\
+                   TL.has_next_add_of_key itsl i (key_of (I.index itsl i))))
+        (ensures (is_blum_add (I.index itsl (TL.next_add_of_key itsl i (key_of (I.index itsl i)))) /\
                   blum_evict_elem itsl i =                                   
-                  blum_add_elem (index itsl (TL.next_add_of_key itsl i (TL.key_of (index itsl i)))))) = 
-  admit()                  
+                  blum_add_elem (I.index itsl (TL.next_add_of_key itsl i (key_of (I.index itsl i)))))) = admit()
 
-let lemma_eac_evicted_blum_implies_previous_evict (#p:pos) (itsl: its_log p) (k:key):
+(* when the eac store is evicted, there exists a previous evict *)
+let lemma_eac_evicted_blum_implies_previous_evict (itsl: its_log) (k:key):
   Lemma (requires (is_eac_state_evicted_blum itsl k))
         (ensures (has_some_entry_of_key itsl k /\
-                  is_blum_evict (index itsl (last_idx_of_key itsl k)) /\
+                  is_evict_to_blum (I.index itsl (last_idx_of_key itsl k)) /\
                   blum_evict_elem itsl (last_idx_of_key itsl k) = 
                   to_blum_elem (eac_state_of_key itsl k) k)) = admit()
 
 (* if we provide two indexes having the same add element then the membership of the element in the 
  * add set is at least two *)
-let lemma_add_set_mem (#p:pos) (itsl: its_log p) (i: seq_index itsl) (j:seq_index itsl{j <> i}):
-  Lemma (requires (is_blum_add (index itsl i) /\
-                   is_blum_add (index itsl j) /\
-                   blum_add_elem (index itsl i) = blum_add_elem (index itsl j)))
-        (ensures (MS.mem (blum_add_elem (index itsl i)) (ts_add_set itsl) >= 2)) = admit()
+let lemma_add_set_mem (itsl: its_log) (i: I.seq_index itsl) (j:I.seq_index itsl{j <> i}):
+  Lemma (requires (is_blum_add (I.index itsl i) /\
+                   is_blum_add (I.index itsl j) /\
+                   blum_add_elem (I.index itsl i) = blum_add_elem (I.index itsl j)))
+        (ensures (MS.mem (blum_add_elem (I.index itsl i)) (ts_add_set itsl) >= 2)) = admit()
